src/DY.Core.Trace.Invariant.fst
@@ -7,7 +7,7 @@ open DY.Core.Label.Type
 open DY.Core.Label
 
 noeq
-type state_predicate (cpreds:crypto_predicates) = {
+type state_predicate (cinvs:crypto_invariants) = {
   pred: trace -> principal -> nat -> bytes -> prop;
   // TODO: Do we want the later lemma?
   pred_later:
@@ -23,37 +23,37 @@ type state_predicate (cpreds:crypto_predicates) = {
     Lemma
     (requires pred tr prin sess_id content)
     (ensures
-      is_knowable_by cpreds (principal_state_label prin sess_id) tr content
+      is_knowable_by cinvs (principal_state_label prin sess_id) tr content
     )
   ;
 }
 
 noeq
-type trace_predicates (cpreds:crypto_predicates) = {
-  state_pred: state_predicate cpreds;
+type trace_invariants (cinvs:crypto_invariants) = {
+  state_pred: state_predicate cinvs;
   event_pred: trace -> principal -> string -> bytes -> prop;
 }
 
 noeq
-type protocol_predicates = {
-  crypto_preds: crypto_predicates;
-  trace_preds: trace_predicates crypto_preds;
+type protocol_invariants = {
+  crypto_invs: crypto_invariants;
+  trace_invs: trace_invariants crypto_invs;
 }
 
-val trace_invariant: protocol_predicates -> trace -> prop
-let rec trace_invariant preds tr =
+val trace_invariant: protocol_invariants -> trace -> prop
+let rec trace_invariant invs tr =
   match tr with
   | Nil -> True
   | Snoc tr_init event ->
-    trace_invariant preds tr_init /\ (
+    trace_invariant invs tr_init /\ (
       match event with
       | MsgSent msg ->
-        is_publishable preds.crypto_preds tr msg
+        is_publishable invs.crypto_invs tr msg
       | SetState prin sess_id content -> (
-        preds.trace_preds.state_pred.pred tr_init prin sess_id content
+        invs.trace_invs.state_pred.pred tr_init prin sess_id content
       )
       | Event prin tag content -> (
-        preds.trace_preds.event_pred tr_init prin tag content
+        invs.trace_invs.event_pred tr_init prin tag content
       )
       | _ -> True
     )
@@ -63,85 +63,85 @@ let rec trace_invariant preds tr =
 
 // Lemma for attacker theorem
 val msg_sent_on_network_are_publishable:
-  preds:protocol_predicates -> tr:trace -> msg:bytes ->
+  invs:protocol_invariants -> tr:trace -> msg:bytes ->
   Lemma
   (requires
-    trace_invariant preds tr /\
+    trace_invariant invs tr /\
     msg_sent_on_network tr msg
   )
-  (ensures is_publishable preds.crypto_preds tr msg)
-let rec msg_sent_on_network_are_publishable preds tr msg =
+  (ensures is_publishable invs.crypto_invs tr msg)
+let rec msg_sent_on_network_are_publishable invs tr msg =
   match tr with
   | Nil -> assert(False)
   | Snoc tr_init (MsgSent msg') -> (
     assert(tr_init <$ tr);
     if msg = msg' then ()
     else (
-      msg_sent_on_network_are_publishable preds tr_init msg
+      msg_sent_on_network_are_publishable invs tr_init msg
     )
   )
   | Snoc tr_init _ ->
     assert(tr_init <$ tr);
-    msg_sent_on_network_are_publishable preds tr_init msg
+    msg_sent_on_network_are_publishable invs tr_init msg
 
 
 val state_was_set_implies_pred:
-  preds:protocol_predicates -> tr:trace ->
+  invs:protocol_invariants -> tr:trace ->
   prin:principal -> sess_id:nat -> content:bytes ->
   Lemma
   (requires
-    trace_invariant preds tr /\
+    trace_invariant invs tr /\
     state_was_set tr prin sess_id content
   )
-  (ensures preds.trace_preds.state_pred.pred tr prin sess_id content)
+  (ensures invs.trace_invs.state_pred.pred tr prin sess_id content)
   [SMTPat (state_was_set tr prin sess_id content);
-   SMTPat (trace_invariant preds tr);
+   SMTPat (trace_invariant invs tr);
   ]
-let rec state_was_set_implies_pred preds tr prin sess_id content =
+let rec state_was_set_implies_pred invs tr prin sess_id content =
   match tr with
   | Nil -> assert(False)
   | Snoc tr_init (SetState prin' sess_id' content') -> (
     assert(tr_init <$ tr);
     if prin = prin' && sess_id = sess_id' && content = content' then (
-      preds.trace_preds.state_pred.pred_later tr_init tr prin sess_id content
+      invs.trace_invs.state_pred.pred_later tr_init tr prin sess_id content
     ) else (
-      state_was_set_implies_pred preds tr_init prin sess_id content;
-      preds.trace_preds.state_pred.pred_later tr_init tr prin sess_id content
+      state_was_set_implies_pred invs tr_init prin sess_id content;
+      invs.trace_invs.state_pred.pred_later tr_init tr prin sess_id content
     )
   )
   | Snoc tr_init _ ->
     assert(tr_init <$ tr);
-    state_was_set_implies_pred preds tr_init prin sess_id content;
-    preds.trace_preds.state_pred.pred_later tr_init tr prin sess_id content
+    state_was_set_implies_pred invs tr_init prin sess_id content;
+    invs.trace_invs.state_pred.pred_later tr_init tr prin sess_id content
 
 // Lemma for attacker theorem
 val state_is_knowable_by:
-  preds:protocol_predicates -> tr:trace ->
+  invs:protocol_invariants -> tr:trace ->
   prin:principal -> sess_id:nat -> content:bytes ->
   Lemma
   (requires
-    trace_invariant preds tr /\
+    trace_invariant invs tr /\
     state_was_set tr prin sess_id content
   )
-  (ensures is_knowable_by preds.crypto_preds (principal_state_label prin sess_id) tr content)
-let state_is_knowable_by preds tr prin sess_id content =
-  preds.trace_preds.state_pred.pred_knowable tr prin sess_id content
+  (ensures is_knowable_by invs.crypto_invs (principal_state_label prin sess_id) tr content)
+let state_is_knowable_by invs tr prin sess_id content =
+  invs.trace_invs.state_pred.pred_knowable tr prin sess_id content
 
 val event_triggered_at_implies_pred:
-  preds:protocol_predicates -> tr:trace ->
+  invs:protocol_invariants -> tr:trace ->
   i:nat -> prin:principal -> tag:string -> content:bytes ->
   Lemma
   (requires
     event_triggered_at tr i prin tag content /\
-    trace_invariant preds tr
+    trace_invariant invs tr
   )
-  (ensures preds.trace_preds.event_pred (prefix tr i) prin tag content)
+  (ensures invs.trace_invs.event_pred (prefix tr i) prin tag content)
   [SMTPat (event_triggered_at tr i prin tag content);
-   SMTPat (trace_invariant preds tr);
+   SMTPat (trace_invariant invs tr);
   ]
-let rec event_triggered_at_implies_pred preds tr i prin tag content =
+let rec event_triggered_at_implies_pred invs tr i prin tag content =
   if i+1 = DY.Core.Trace.Type.length tr then ()
   else (
     let Snoc tr_init _ = tr in
-    event_triggered_at_implies_pred preds tr_init i prin tag content
+    event_triggered_at_implies_pred invs tr_init i prin tag content
   )
