src/DY.Example.NSL.Protocol.Stateful.Proof.fst
@@ -12,34 +12,34 @@ open DY.Example.NSL.Protocol.Stateful
 (*** Trace predicates ***)
 
 let nsl_session_pred: typed_session_pred nsl_session = {
-  pred = (fun cpreds tr prin sess_id st ->
+  pred = (fun cinvs tr prin sess_id st ->
     match st with
     | InitiatorSentMsg1 bob n_a -> (
       let alice = prin in
-      is_knowable_by cpreds (join (principal_label alice) (principal_label bob)) tr n_a /\
+      is_knowable_by cinvs (join (principal_label alice) (principal_label bob)) tr n_a /\
       event_triggered tr alice nsl_event_label (serialize nsl_event (Initiate1 alice bob n_a))
     )
     | ResponderSentMsg2 alice n_a n_b -> (
       let bob = prin in
-      is_knowable_by cpreds (join (principal_label alice) (principal_label bob)) tr n_a /\
-      is_knowable_by cpreds (join (principal_label alice) (principal_label bob)) tr n_b /\
+      is_knowable_by cinvs (join (principal_label alice) (principal_label bob)) tr n_a /\
+      is_knowable_by cinvs (join (principal_label alice) (principal_label bob)) tr n_b /\
       event_triggered tr bob nsl_event_label (serialize nsl_event (Respond1 alice bob n_a n_b))
     )
     | InitiatorSentMsg3 bob n_a n_b  -> (
       let alice = prin in
-      is_knowable_by cpreds (join (principal_label alice) (principal_label bob)) tr n_a /\
-      is_knowable_by cpreds (join (principal_label alice) (principal_label bob)) tr n_b /\
+      is_knowable_by cinvs (join (principal_label alice) (principal_label bob)) tr n_a /\
+      is_knowable_by cinvs (join (principal_label alice) (principal_label bob)) tr n_b /\
       event_triggered tr alice nsl_event_label (serialize nsl_event (Initiate2 alice bob n_a n_b))
     )
     | ResponderReceivedMsg3 alice n_a n_b -> (
       let bob = prin in
-      is_knowable_by cpreds (join (principal_label alice) (principal_label bob)) tr n_a /\
-      is_knowable_by cpreds (join (principal_label alice) (principal_label bob)) tr n_b /\
+      is_knowable_by cinvs (join (principal_label alice) (principal_label bob)) tr n_a /\
+      is_knowable_by cinvs (join (principal_label alice) (principal_label bob)) tr n_b /\
       event_triggered tr bob nsl_event_label (serialize nsl_event (Respond2 alice bob n_a n_b))
     )
   );
-  pred_later = (fun cpreds tr1 tr2 prin sess_id st -> ());
-  pred_knowable = (fun cpreds tr prin sess_id st -> ());
+  pred_later = (fun cinvs tr1 tr2 prin sess_id st -> ());
+  pred_knowable = (fun cinvs tr prin sess_id st -> ());
 }
 
 let all_sessions = [
@@ -48,11 +48,11 @@ let all_sessions = [
   (nsl_session_label, typed_session_pred_to_session_pred nsl_session_pred);
 ]
 
-val full_nsl_session_pred: state_predicate nsl_crypto_preds
+val full_nsl_session_pred: state_predicate nsl_crypto_invs
 let full_nsl_session_pred =
-  mk_state_predicate nsl_crypto_preds all_sessions
+  mk_state_predicate nsl_crypto_invs all_sessions
 
-let nsl_trace_preds: trace_predicates (nsl_crypto_preds) = {
+let nsl_trace_invs: trace_invariants (nsl_crypto_invs) = {
   state_pred = full_nsl_session_pred;
   event_pred = (fun tr prin evt_label evt ->
     evt_label == nsl_event_label /\ (
@@ -88,9 +88,9 @@ let nsl_trace_preds: trace_predicates (nsl_crypto_preds) = {
   );
 }
 
-let nsl_protocol_preds: protocol_predicates = {
-  crypto_preds = nsl_crypto_preds;
-  trace_preds = nsl_trace_preds;
+let nsl_protocol_invs: protocol_invariants = {
+  crypto_invs = nsl_crypto_invs;
+  trace_invs = nsl_trace_invs;
 }
 
 inline_for_extraction noextract
@@ -98,29 +98,29 @@ val session_memP_tactic: unit -> FStar.Tactics.Tac unit
 let session_memP_tactic () =
   FStar.Tactics.norm [delta_only [`%List.Tot.Base.memP; `%all_sessions]; iota; zeta]
 
-val full_nsl_session_pred_has_pki_invariant: squash (has_pki_invariant nsl_protocol_preds)
+val full_nsl_session_pred_has_pki_invariant: squash (has_pki_invariant nsl_protocol_invs)
 let full_nsl_session_pred_has_pki_invariant =
   let lab = pki_label in
   let spred = typed_session_pred_to_session_pred (map_session_invariant pki_pred) in
   assert_norm(List.Tot.no_repeats_p (List.Tot.map fst (all_sessions)));
   assert(List.Tot.memP (lab, spred) (all_sessions)) by (session_memP_tactic());
-  mk_global_session_pred_correct nsl_protocol_preds (all_sessions) lab spred
+  mk_global_session_pred_correct nsl_protocol_invs (all_sessions) lab spred
 
-val full_nsl_session_pred_has_private_keys_invariant: squash (has_private_keys_invariant nsl_protocol_preds)
+val full_nsl_session_pred_has_private_keys_invariant: squash (has_private_keys_invariant nsl_protocol_invs)
 let full_nsl_session_pred_has_private_keys_invariant =
   let lab = private_keys_label in
   let spred = typed_session_pred_to_session_pred (map_session_invariant private_keys_pred) in
   assert_norm(List.Tot.no_repeats_p (List.Tot.map fst (all_sessions)));
   assert(List.Tot.memP (lab, spred) (all_sessions)) by (session_memP_tactic());
-  mk_global_session_pred_correct nsl_protocol_preds (all_sessions) lab spred
+  mk_global_session_pred_correct nsl_protocol_invs (all_sessions) lab spred
 
-val full_nsl_session_pred_has_nsl_invariant: squash (has_typed_session_pred nsl_protocol_preds nsl_session_label nsl_session_pred)
+val full_nsl_session_pred_has_nsl_invariant: squash (has_typed_session_pred nsl_protocol_invs nsl_session_label nsl_session_pred)
 let full_nsl_session_pred_has_nsl_invariant =
   let lab = nsl_session_label in
   let spred = typed_session_pred_to_session_pred nsl_session_pred in
   assert_norm(List.Tot.no_repeats_p (List.Tot.map fst (all_sessions)));
   assert(List.Tot.memP (lab, spred) (all_sessions)) by (session_memP_tactic());
-  mk_global_session_pred_correct nsl_protocol_preds (all_sessions) lab spred
+  mk_global_session_pred_correct nsl_protocol_invs (all_sessions) lab spred
 
 (*** Proof ***)
 
@@ -128,10 +128,10 @@ val prepare_msg1_proof:
   tr:trace ->
   alice:principal -> bob:principal ->
   Lemma
-  (requires trace_invariant nsl_protocol_preds tr)
+  (requires trace_invariant nsl_protocol_invs tr)
   (ensures (
     let (sess_id, tr_out) = prepare_msg1 alice bob tr in
-    trace_invariant nsl_protocol_preds tr
+    trace_invariant nsl_protocol_invs tr
   ))
 let prepare_msg1_proof tr alice bob =
   ()
@@ -140,12 +140,12 @@ val send_msg1_proof:
   tr:trace ->
   global_sess_id:nsl_global_sess_ids -> alice:principal -> sess_id:nat ->
   Lemma
-  (requires trace_invariant nsl_protocol_preds tr)
+  (requires trace_invariant nsl_protocol_invs tr)
   (ensures (
     let (opt_msg_id, tr_out) = send_msg1 global_sess_id alice sess_id tr in
     match opt_msg_id with
     | None -> True
-    | Some msg_id -> trace_invariant nsl_protocol_preds tr_out
+    | Some msg_id -> trace_invariant nsl_protocol_invs tr_out
   ))
 let send_msg1_proof tr global_sess_id alice sess_id =
   let (opt_msg_id, tr_out) = send_msg1 global_sess_id alice sess_id tr in
@@ -165,12 +165,12 @@ val prepare_msg2_proof:
   tr:trace ->
   global_sess_id:nsl_global_sess_ids -> bob:principal -> msg_id:nat ->
   Lemma
-  (requires trace_invariant nsl_protocol_preds tr)
+  (requires trace_invariant nsl_protocol_invs tr)
   (ensures (
     let (opt_sess_id, tr_out) = prepare_msg2 global_sess_id bob msg_id tr in
     match opt_sess_id with
     | None -> True
-    | Some sess_id -> trace_invariant nsl_protocol_preds tr_out
+    | Some sess_id -> trace_invariant nsl_protocol_invs tr_out
   ))
 let prepare_msg2_proof tr global_sess_id bob msg_id =
   let (opt_sess_id, tr_out) = prepare_msg2 global_sess_id bob msg_id tr in
@@ -191,12 +191,12 @@ val send_msg2_proof:
   tr:trace ->
   global_sess_id:nsl_global_sess_ids -> bob:principal -> sess_id:nat ->
   Lemma
-  (requires trace_invariant nsl_protocol_preds tr)
+  (requires trace_invariant nsl_protocol_invs tr)
   (ensures (
     let (opt_msg_id, tr_out) = send_msg2 global_sess_id bob sess_id tr in
     match opt_msg_id with
     | None -> True
-    | Some msg_id -> trace_invariant nsl_protocol_preds tr_out
+    | Some msg_id -> trace_invariant nsl_protocol_invs tr_out
   ))
 let send_msg2_proof tr global_sess_id bob sess_id =
   let (opt_msg_id, tr_out) = send_msg2 global_sess_id bob sess_id tr in
@@ -217,12 +217,12 @@ val prepare_msg3_proof:
   tr:trace ->
   global_sess_id:nsl_global_sess_ids -> alice:principal -> sess_id:nat -> msg_id:nat ->
   Lemma
-  (requires trace_invariant nsl_protocol_preds tr)
+  (requires trace_invariant nsl_protocol_invs tr)
   (ensures (
     let (opt_sess_id, tr_out) = prepare_msg3 global_sess_id alice sess_id msg_id tr in
     match opt_sess_id with
     | None -> True
-    | Some sess_id -> trace_invariant nsl_protocol_preds tr_out
+    | Some sess_id -> trace_invariant nsl_protocol_invs tr_out
   ))
 let prepare_msg3_proof tr global_sess_id alice sess_id msg_id =
   let (opt_sess_id, tr_out) = prepare_msg3 global_sess_id alice sess_id msg_id tr in
@@ -246,12 +246,12 @@ val send_msg3_proof:
   tr:trace ->
   global_sess_id:nsl_global_sess_ids -> alice:principal -> sess_id:nat ->
   Lemma
-  (requires trace_invariant nsl_protocol_preds tr)
+  (requires trace_invariant nsl_protocol_invs tr)
   (ensures (
     let (opt_msg_id, tr_out) = send_msg3 global_sess_id alice sess_id tr in
     match opt_msg_id with
     | None -> True
-    | Some msg_id -> trace_invariant nsl_protocol_preds tr_out
+    | Some msg_id -> trace_invariant nsl_protocol_invs tr_out
   ))
 let send_msg3_proof tr global_sess_id alice sess_id =
   let (opt_msg_id, tr_out) = send_msg3 global_sess_id alice sess_id tr in
@@ -274,7 +274,7 @@ val event_respond1_injective:
   n_a:bytes -> n_a':bytes -> n_b:bytes ->
   Lemma
   (requires
-    trace_invariant nsl_protocol_preds tr /\
+    trace_invariant nsl_protocol_invs tr /\
     event_triggered tr bob nsl_event_label (serialize nsl_event (Respond1 alice bob n_a n_b)) /\
     event_triggered tr bob nsl_event_label (serialize nsl_event (Respond1 alice' bob n_a' n_b))
   )
@@ -290,12 +290,12 @@ val prepare_msg4:
   tr:trace ->
   global_sess_id:nsl_global_sess_ids -> bob:principal -> sess_id:nat -> msg_id:nat ->
   Lemma
-  (requires trace_invariant nsl_protocol_preds tr)
+  (requires trace_invariant nsl_protocol_invs tr)
   (ensures (
     let (opt_sess_id, tr_out) = prepare_msg4 global_sess_id bob sess_id msg_id tr in
     match opt_sess_id with
     | None -> True
-    | Some sess_id -> trace_invariant nsl_protocol_preds tr_out
+    | Some sess_id -> trace_invariant nsl_protocol_invs tr_out
   ))
 let prepare_msg4 tr global_sess_id bob sess_id msg_id =
   let (opt_sess_id, tr_out) = prepare_msg4 global_sess_id bob sess_id msg_id tr in
