src/DY.Example.NSL.Protocol.Total.Proof.fst
@@ -8,7 +8,7 @@ open DY.Example.NSL.Protocol.Stateful
 #set-options "--fuel 0 --ifuel 0"
 
 #push-options "--ifuel 2 --fuel 0"
-let nsl_crypto_preds = {
+let nsl_crypto_invs = {
   aead_pred = (fun tr key nonce msg ad -> False);
   aead_pred_later = (fun tr1 tr2 key nonce msg ad -> ());
 
@@ -49,19 +49,19 @@ val compute_message1_proof:
     // From the stateful code
     event_triggered tr alice nsl_event_label (serialize nsl_event (Initiate1 alice bob n_a)) /\
     // From random generation
-    is_secret nsl_crypto_preds (join (principal_label alice) (principal_label bob)) tr n_a  /\
+    is_secret nsl_crypto_invs (join (principal_label alice) (principal_label bob)) tr n_a  /\
     // From random generation
-    is_secret nsl_crypto_preds (principal_label alice) tr nonce /\
+    is_secret nsl_crypto_invs (principal_label alice) tr nonce /\
     // From PKI invariants
-    is_encryption_key nsl_crypto_preds (principal_label bob) tr pk_b
+    is_encryption_key nsl_crypto_invs (principal_label bob) tr pk_b
   )
-  (ensures is_publishable nsl_crypto_preds tr (compute_message1 alice bob pk_b n_a nonce))
+  (ensures is_publishable nsl_crypto_invs tr (compute_message1 alice bob pk_b n_a nonce))
 let compute_message1_proof tr alice bob pk_b n_a nonce =
   // trigger `join_eq` SMTPat
   assert (join (principal_label alice) (principal_label bob) `can_flow tr` join (principal_label alice) (principal_label bob));
   let msg = Msg1 {n_a; alice;} in
-  serialize_wf_lemma message (is_knowable_by nsl_crypto_preds (principal_label alice) tr) msg;
-  serialize_wf_lemma message (is_knowable_by nsl_crypto_preds (principal_label bob) tr) msg
+  serialize_wf_lemma message (is_knowable_by nsl_crypto_invs (principal_label alice) tr) msg;
+  serialize_wf_lemma message (is_knowable_by nsl_crypto_invs (principal_label bob) tr) msg
 
 // If bob successfully decrypt the first message,
 // then n_a is knownable both by alice (in the message) and bob (the principal)
@@ -75,15 +75,15 @@ val decode_message1_proof:
   Lemma
   (requires
     // From PrivateKeys invariants
-    is_decryption_key nsl_crypto_preds (principal_label bob) tr sk_b /\
+    is_decryption_key nsl_crypto_invs (principal_label bob) tr sk_b /\
     // From the network
-    bytes_invariant nsl_crypto_preds tr msg_cipher
+    bytes_invariant nsl_crypto_invs tr msg_cipher
   )
   (ensures (
     match decode_message1 bob msg_cipher sk_b with
     | None -> True
     | Some msg1 -> (
-      is_knowable_by nsl_crypto_preds (join (principal_label msg1.alice) (principal_label bob)) tr msg1.n_a
+      is_knowable_by nsl_crypto_invs (join (principal_label msg1.alice) (principal_label bob)) tr msg1.n_a
     )
   ))
 let decode_message1_proof tr bob msg_cipher sk_b =
@@ -92,8 +92,8 @@ let decode_message1_proof tr bob msg_cipher sk_b =
   | Some msg1 ->
     let Some msg = pk_dec sk_b msg_cipher in
     assert(public `can_flow tr` (join (principal_label msg1.alice) (principal_label bob)));
-    FStar.Classical.move_requires (parse_wf_lemma message (is_publishable nsl_crypto_preds tr)) msg;
-    FStar.Classical.move_requires (parse_wf_lemma message (bytes_invariant nsl_crypto_preds tr)) msg
+    FStar.Classical.move_requires (parse_wf_lemma message (is_publishable nsl_crypto_invs tr)) msg;
+    FStar.Classical.move_requires (parse_wf_lemma message (bytes_invariant nsl_crypto_invs tr)) msg
 #pop-options
 
 val compute_message2_proof:
@@ -104,22 +104,22 @@ val compute_message2_proof:
     // From the stateful code
     event_triggered tr bob nsl_event_label (serialize nsl_event (Respond1 msg1.alice bob msg1.n_a n_b)) /\
     // From decode_message1_proof
-    is_knowable_by nsl_crypto_preds (join (principal_label msg1.alice) (principal_label bob)) tr msg1.n_a /\
+    is_knowable_by nsl_crypto_invs (join (principal_label msg1.alice) (principal_label bob)) tr msg1.n_a /\
     // From the random generation
-    is_secret nsl_crypto_preds (join (principal_label msg1.alice) (principal_label bob)) tr n_b /\
+    is_secret nsl_crypto_invs (join (principal_label msg1.alice) (principal_label bob)) tr n_b /\
     // From the random generation
-    is_secret nsl_crypto_preds (principal_label bob) tr nonce /\
+    is_secret nsl_crypto_invs (principal_label bob) tr nonce /\
     // From the PKI
-    is_encryption_key nsl_crypto_preds (principal_label msg1.alice) tr pk_a
+    is_encryption_key nsl_crypto_invs (principal_label msg1.alice) tr pk_a
   )
   (ensures
-    is_publishable nsl_crypto_preds tr (compute_message2 bob msg1 pk_a n_b nonce)
+    is_publishable nsl_crypto_invs tr (compute_message2 bob msg1 pk_a n_b nonce)
   )
 let compute_message2_proof tr bob msg1 pk_a n_b nonce =
   assert (join (principal_label msg1.alice) (principal_label bob) `can_flow tr` join (principal_label msg1.alice) (principal_label bob));
   let msg = Msg2 {n_a = msg1.n_a;  n_b; bob;} in
-  serialize_wf_lemma message (is_knowable_by nsl_crypto_preds (principal_label msg1.alice) tr) msg;
-  serialize_wf_lemma message (is_knowable_by nsl_crypto_preds (principal_label bob) tr) msg
+  serialize_wf_lemma message (is_knowable_by nsl_crypto_invs (principal_label msg1.alice) tr) msg;
+  serialize_wf_lemma message (is_knowable_by nsl_crypto_invs (principal_label bob) tr) msg
 
 // If alice successfully decrypt the second message,
 // then n_b is knownable both by alice (in the message) and bob (the principal)
@@ -133,17 +133,17 @@ val decode_message2_proof:
   Lemma
   (requires
     // From the NSL state invariant
-    is_secret nsl_crypto_preds (join (principal_label alice) (principal_label bob)) tr n_a /\
+    is_secret nsl_crypto_invs (join (principal_label alice) (principal_label bob)) tr n_a /\
     // From the PrivateKeys invariant
-    is_decryption_key nsl_crypto_preds (principal_label alice) tr sk_a /\
+    is_decryption_key nsl_crypto_invs (principal_label alice) tr sk_a /\
     // From the network
-    bytes_invariant nsl_crypto_preds tr msg_cipher
+    bytes_invariant nsl_crypto_invs tr msg_cipher
   )
   (ensures (
     match decode_message2 alice bob msg_cipher sk_a n_a with
     | None -> True
     | Some msg2 -> (
-      is_knowable_by nsl_crypto_preds (join (principal_label alice) (principal_label bob)) tr msg2.n_b /\ (
+      is_knowable_by nsl_crypto_invs (join (principal_label alice) (principal_label bob)) tr msg2.n_b /\ (
       (principal_corrupt tr alice \/ principal_corrupt tr bob) \/ (
         event_triggered tr bob nsl_event_label (serialize nsl_event (Respond1 alice bob n_a msg2.n_b))
       )
@@ -158,8 +158,8 @@ let decode_message2_proof tr alice bob msg_cipher sk_a n_a =
     let Some msg = pk_dec sk_a msg_cipher in
     let Some msg2' = parse message msg in
     let Msg2 msg2' = msg2' in
-    FStar.Classical.move_requires (parse_wf_lemma message (is_publishable nsl_crypto_preds tr)) msg;
-    FStar.Classical.move_requires (parse_wf_lemma message (bytes_invariant nsl_crypto_preds tr)) msg
+    FStar.Classical.move_requires (parse_wf_lemma message (is_publishable nsl_crypto_invs tr)) msg;
+    FStar.Classical.move_requires (parse_wf_lemma message (bytes_invariant nsl_crypto_invs tr)) msg
   )
 #pop-options
 
@@ -171,21 +171,21 @@ val compute_message3_proof:
     // From the stateful code
     (exists n_a. event_triggered tr alice nsl_event_label (serialize nsl_event (Initiate2 alice bob n_a n_b))) /\
     // From decode_message2_proof
-    is_knowable_by nsl_crypto_preds (join (principal_label alice) (principal_label bob)) tr n_b /\
+    is_knowable_by nsl_crypto_invs (join (principal_label alice) (principal_label bob)) tr n_b /\
     // From the random generation
-    is_secret nsl_crypto_preds (principal_label alice) tr nonce /\
+    is_secret nsl_crypto_invs (principal_label alice) tr nonce /\
     // From the PKI
-    is_encryption_key nsl_crypto_preds (principal_label bob) tr pk_b
+    is_encryption_key nsl_crypto_invs (principal_label bob) tr pk_b
   )
   (ensures
-    is_publishable nsl_crypto_preds tr (compute_message3 alice bob pk_b n_b nonce)
+    is_publishable nsl_crypto_invs tr (compute_message3 alice bob pk_b n_b nonce)
   )
 let compute_message3_proof tr alice bob pk_b n_b nonce =
   assert (join (principal_label alice) (principal_label bob) `can_flow tr` join (principal_label alice) (principal_label bob));
   assert(exists alice n_a. event_triggered tr alice nsl_event_label (serialize nsl_event (Initiate2 alice bob n_a n_b)));
   let msg = Msg3 {n_b;} in
-  serialize_wf_lemma message (is_knowable_by nsl_crypto_preds (principal_label alice) tr) msg;
-  serialize_wf_lemma message (is_knowable_by nsl_crypto_preds (principal_label bob) tr) msg;
+  serialize_wf_lemma message (is_knowable_by nsl_crypto_invs (principal_label alice) tr) msg;
+  serialize_wf_lemma message (is_knowable_by nsl_crypto_invs (principal_label bob) tr) msg;
   let msg3: message3 = {n_b;} in
   assert(msg3.n_b == n_b)
 
@@ -201,9 +201,9 @@ val decode_message3_proof:
     // From the NSL state invariant
     get_label n_b = join (principal_label alice) (principal_label bob) /\
     // From the PrivateKeys invariant
-    is_decryption_key nsl_crypto_preds (principal_label bob) tr sk_b /\
+    is_decryption_key nsl_crypto_invs (principal_label bob) tr sk_b /\
     // From the network
-    bytes_invariant nsl_crypto_preds tr msg_cipher
+    bytes_invariant nsl_crypto_invs tr msg_cipher
   )
   (ensures (
     match decode_message3 alice bob msg_cipher sk_b n_b with
@@ -221,7 +221,7 @@ let decode_message3_proof tr alice bob msg_cipher sk_b n_b =
   | None -> ()
   | Some msg3 -> (
     let Some msg = pk_dec sk_b msg_cipher in
-    FStar.Classical.move_requires (parse_wf_lemma message (is_publishable nsl_crypto_preds tr)) msg;
-    FStar.Classical.move_requires (parse_wf_lemma message (bytes_invariant nsl_crypto_preds tr)) msg
+    FStar.Classical.move_requires (parse_wf_lemma message (is_publishable nsl_crypto_invs tr)) msg;
+    FStar.Classical.move_requires (parse_wf_lemma message (bytes_invariant nsl_crypto_invs tr)) msg
   )
 #pop-options
