src/DY.Lib.State.PKI.fst
@@ -40,30 +40,30 @@ let pki_types = {
 }
 
 val is_public_key_for:
-  crypto_predicates -> trace ->
+  crypto_invariants -> trace ->
   bytes -> public_key_type -> principal -> prop
-let is_public_key_for cpreds tr pk pk_type who =
+let is_public_key_for cinvs tr pk pk_type who =
     match pk_type with
     | PkEnc -> (
-      is_encryption_key cpreds (principal_label who) tr pk
+      is_encryption_key cinvs (principal_label who) tr pk
     )
     | Verify -> (
-      is_verification_key cpreds (principal_label who) tr pk
+      is_verification_key cinvs (principal_label who) tr pk
     )
 
 val pki_pred: map_predicate pki_types
 let pki_pred = {
-  pred = (fun cpreds tr prin sess_id (key:pki_types.key) value ->
-    is_public_key_for cpreds tr value.public_key key.ty key.who
+  pred = (fun cinvs tr prin sess_id (key:pki_types.key) value ->
+    is_public_key_for cinvs tr value.public_key key.ty key.who
   );
-  pred_later = (fun cpreds tr1 tr2 prin sess_id key value -> ());
-  pred_knowable = (fun cpreds tr prin sess_id key value -> ());
+  pred_later = (fun cinvs tr1 tr2 prin sess_id key value -> ());
+  pred_knowable = (fun cinvs tr prin sess_id key value -> ());
 }
 
 val pki_label: string
 let pki_label = "DY.Lib.State.PKI"
 
-val has_pki_invariant: protocol_predicates -> prop
+val has_pki_invariant: protocol_invariants -> prop
 let has_pki_invariant pr =
   has_map_session_invariant pki_pred pki_label pr
 
@@ -82,47 +82,47 @@ let get_public_key prin sess_id pk_type who =
   return (Some res.public_key)
 
 val initialize_pki_invariant:
-  preds:protocol_predicates ->
+  invs:protocol_invariants ->
   prin:principal -> tr:trace ->
   Lemma
   (requires
-    trace_invariant preds tr /\
-    has_pki_invariant preds
+    trace_invariant invs tr /\
+    has_pki_invariant invs
   )
   (ensures (
     let (_, tr_out) = initialize_pki prin tr in
-    trace_invariant preds tr_out
+    trace_invariant invs tr_out
   ))
   [SMTPat (initialize_pki prin tr);
-   SMTPat (has_pki_invariant preds);
-   SMTPat (trace_invariant preds tr)]
-let initialize_pki_invariant preds prin tr = ()
+   SMTPat (has_pki_invariant invs);
+   SMTPat (trace_invariant invs tr)]
+let initialize_pki_invariant invs prin tr = ()
 
 val install_public_key_invariant:
-  preds:protocol_predicates ->
+  invs:protocol_invariants ->
   prin:principal -> sess_id:nat -> pk_type:public_key_type -> who:principal -> pk:bytes -> tr:trace ->
   Lemma
   (requires
-    is_public_key_for preds.crypto_preds tr pk pk_type who /\
-    trace_invariant preds tr /\
-    has_pki_invariant preds
+    is_public_key_for invs.crypto_invs tr pk pk_type who /\
+    trace_invariant invs tr /\
+    has_pki_invariant invs
   )
   (ensures (
     let (_, tr_out) = install_public_key prin sess_id pk_type who pk tr in
-    trace_invariant preds tr_out
+    trace_invariant invs tr_out
   ))
   [SMTPat (install_public_key prin sess_id pk_type who pk tr);
-   SMTPat (has_pki_invariant preds);
-   SMTPat (trace_invariant preds tr)]
-let install_public_key_invariant preds prin sess_id pk_type who pk tr = ()
+   SMTPat (has_pki_invariant invs);
+   SMTPat (trace_invariant invs tr)]
+let install_public_key_invariant invs prin sess_id pk_type who pk tr = ()
 
 val get_public_key_invariant:
-  preds:protocol_predicates ->
+  invs:protocol_invariants ->
   prin:principal -> sess_id:nat -> pk_type:public_key_type -> who:principal -> tr:trace ->
   Lemma
   (requires
-    trace_invariant preds tr /\
-    has_pki_invariant preds
+    trace_invariant invs tr /\
+    has_pki_invariant invs
   )
   (ensures (
     let (opt_public_key, tr_out) = get_public_key prin sess_id pk_type who tr in
@@ -130,10 +130,10 @@ val get_public_key_invariant:
       match opt_public_key with
       | None -> True
       | Some public_key ->
-        is_public_key_for preds.crypto_preds tr public_key pk_type who
+        is_public_key_for invs.crypto_invs tr public_key pk_type who
     )
   ))
   [SMTPat (get_public_key prin sess_id pk_type who tr);
-   SMTPat (has_pki_invariant preds);
-   SMTPat (trace_invariant preds tr)]
-let get_public_key_invariant preds prin sess_id pk_type who tr = ()
+   SMTPat (has_pki_invariant invs);
+   SMTPat (trace_invariant invs tr)]
+let get_public_key_invariant invs prin sess_id pk_type who tr = ()
